Address comments

Strata/DL/Lambda/Semantics.lean
@@ -27,111 +27,110 @@ This small-step definitions faithfully follows the behavior of LExpr.eval,
 except that this inductive definition may stuck early when there is no
 assignment to a free variable available in LState.
 -/
-inductive Step
-  : LState IDMeta → LExpr LMonoTy IDMeta → LExpr LMonoTy IDMeta → Prop where
+inductive Step (F:@Factory IDMeta) (state:Scopes IDMeta)
+  : LExpr LMonoTy IDMeta → LExpr LMonoTy IDMeta → Prop where
 -- A free variable. Stuck if fvar does not exist in LState.
 | expand_fvar:
-  ∀ (σ:LState IDMeta) (x:Identifier IDMeta) (e:LExpr LMonoTy IDMeta),
-    σ.state.find? x = .some (ty,e) →
-    Step σ (.fvar x ty') e
+  ∀ (x:Identifier IDMeta) (e:LExpr LMonoTy IDMeta),
+    state.find? x = .some (ty,e) →
+    Step F state (.fvar x ty') e
 
 -- Beta reduction for lambda; Call-by-value semantics.
 | beta:
-  ∀ (σ:LState IDMeta) (e1 v2:LExpr LMonoTy IDMeta),
-    LExpr.isCanonicalValue σ v2 →
-    Step σ (.app (.abs ty e1) v2) (LExpr.subst v2 e1)
-
--- Universal quantification.
-| beta_univ:
-  ∀ (σ:LState IDMeta) (e1 v2 trig:LExpr LMonoTy IDMeta),
-    LExpr.isCanonicalValue σ v2 →
-    Step σ (.app (.quant .all ty trig e1) v2) (LExpr.subst v2 e1)
+  ∀ (e1 v2:LExpr LMonoTy IDMeta),
+    LExpr.isCanonicalValue F v2 →
+    Step F state (.app (.abs ty e1) v2) (LExpr.subst v2 e1)
 
 -- Call-by-value semantics.
 | reduce_2:
-  ∀ (σ:LState IDMeta) (v1 e2 e2':LExpr LMonoTy IDMeta),
-    LExpr.isCanonicalValue σ v1 →
-    Step σ e2 e2' →
-    Step σ (.app v1 e2) (.app v1 e2')
+  ∀ (v1 e2 e2':LExpr LMonoTy IDMeta),
+    LExpr.isCanonicalValue F v1 →
+    Step F state e2 e2' →
+    Step F state (.app v1 e2) (.app v1 e2')
 
 | reduce_1:
-  ∀ (σ:LState IDMeta) (e1 e1' e2:LExpr LMonoTy IDMeta),
-    Step σ e1 e1' →
-    Step σ (.app e1 e2) (.app e1' e2)
+  ∀ (e1 e1' e2:LExpr LMonoTy IDMeta),
+    Step F state  e1 e1' →
+    Step F state  (.app e1 e2) (.app e1' e2)
 
 -- For ite x e1 e2, do not eagerly evaluate e1 and e2.
 -- For the reduction order, ite x e1 e2 is interpreted as
 -- 'ite x (λ.e1) (λ.e2)'.
 | ite_beta_then:
-  ∀ (σ:LState IDMeta) (ethen eelse:LExpr LMonoTy IDMeta),
-    Step σ (.ite (.const (.boolConst true)) ethen eelse) ethen
+  ∀ (ethen eelse:LExpr LMonoTy IDMeta),
+    Step F state  (.ite (.const (.boolConst true)) ethen eelse) ethen
 
 | ite_beta_else:
-  ∀ (σ:LState IDMeta) (ethen eelse:LExpr LMonoTy IDMeta),
-    Step σ (.ite (.const (.boolConst false)) ethen eelse) eelse
+  ∀ (ethen eelse:LExpr LMonoTy IDMeta),
+    Step F state  (.ite (.const (.boolConst false)) ethen eelse) eelse
 
 | ite_reduce_cond:
-  ∀ (σ:LState IDMeta) (econd econd' ethen eelse:LExpr LMonoTy IDMeta),
-    Step σ econd econd' →
-    Step σ (.ite econd ethen eelse) (.ite econd' ethen eelse)
+  ∀ (econd econd' ethen eelse:LExpr LMonoTy IDMeta),
+    Step F state  econd econd' →
+    Step F state  (.ite econd ethen eelse) (.ite econd' ethen eelse)
 
 -- Equality. Reduce after both operands evaluate to values.
 | beta_eq:
-  ∀ (σ:LState IDMeta) (e1 e2:LExpr LMonoTy IDMeta)
-    (H1:LExpr.isCanonicalValue σ e1)
-    (H2:LExpr.isCanonicalValue σ e2),
-    Step σ (.eq e1 e2) (.const (.boolConst (LExpr.eql σ e1 e2 H1 H2)))
+  ∀ (e1 e2 eres:LExpr LMonoTy IDMeta)
+    (H1:LExpr.isCanonicalValue F e1)
+    (H2:LExpr.isCanonicalValue F e2),
+    eres = .const (.boolConst (LExpr.eql F e1 e2 H1 H2)) →
+    Step F state  (.eq e1 e2) eres
 
 | reduce_eq_lhs:
-  ∀ (σ:LState IDMeta) (e1 e1' e2:LExpr LMonoTy IDMeta),
-    Step σ e1 e1' →
-    Step σ (.eq e1 e2) (.eq e1' e2)
+  ∀ (e1 e1' e2:LExpr LMonoTy IDMeta),
+    Step F state  e1 e1' →
+    Step F state  (.eq e1 e2) (.eq e1' e2)
 
 | reduce_eq_rhs:
-  ∀ (σ:LState IDMeta) (v1 e2 e2':LExpr LMonoTy IDMeta),
-    LExpr.isCanonicalValue σ v1 → Step σ e2 e2' →
-    Step σ (.eq v1 e2) (.eq v1 e2')
+  ∀ (v1 e2 e2':LExpr LMonoTy IDMeta),
+    LExpr.isCanonicalValue F v1 →
+    Step F state  e2 e2' →
+    Step F state  (.eq v1 e2) (.eq v1 e2')
 
 -- Evaluation keeps the metadata.
 | mdata:
-  ∀ (σ:LState IDMeta) (e e':LExpr LMonoTy IDMeta) (m:Info),
-    Step σ e e' →
-    Step σ (.mdata m e) (.mdata m e')
+  ∀ (e e':LExpr LMonoTy IDMeta) (m:Info),
+    Step F state  e e' →
+    Step F state  (.mdata m e) (.mdata m e')
 
 -- Expand functions and free variables when they are evaluated.
 -- If the function body is unknown, concreteEval can be instead used. Look at
 -- the eval_fn constructor below.
 -- This is consistent with what LExpr.eval does (modulo the "inline" flag).
 | expand_fn:
-  ∀ (σ:LState IDMeta) (e callee fnbody new_body:LExpr LMonoTy IDMeta) args fn,
-    σ.config.factory.callOfLFunc e = .some (callee,args,fn) →
-    args.all (LExpr.isCanonicalValue σ) →
+  ∀ (e callee fnbody new_body:LExpr LMonoTy IDMeta) args fn,
+    F.callOfLFunc e = .some (callee,args,fn) →
+    args.all (LExpr.isCanonicalValue F) →
     fn.body = .some fnbody →
     new_body = LExpr.substFvars fnbody (fn.inputs.keys.zip args) →
-    Step σ e new_body
+    Step F state  e new_body
 
 -- The second way of evaluating a function call.
 -- If LFunc has a concrete evaluator, this can be used to 'jump' to the final
 -- result of the function.
 | eval_fn:
-  ∀ (σ:LState IDMeta) (e callee:LExpr LMonoTy IDMeta) args fn denotefn,
-    σ.config.factory.callOfLFunc e = .some (callee,args,fn) →
-    args.all (LExpr.isCanonicalValue σ) →
+  ∀ (e callee:LExpr LMonoTy IDMeta) args fn denotefn,
+    F.callOfLFunc e = .some (callee,args,fn) →
+    args.all (LExpr.isCanonicalValue F) →
     fn.concreteEval = .some denotefn →
-    Step σ e (denotefn (LExpr.mkApp callee args) args)
+    Step F state  e (denotefn (LExpr.mkApp callee args) args)
 
 
 theorem step_const_stuck:
-  ∀ (σ:LState IDMeta) x e, ¬ Step σ (.const x) e := by
-  intros σ x e H
+  ∀ (F:@Factory IDMeta) (state:Scopes IDMeta) x e,
+  ¬ Step F state  (.const x) e := by
+  intros
+  intro H
   contradiction
 
 /--
 Multi-step execution: reflexive transitive closure of single steps.
 -/
-inductive StepStar
-  : LState IDMeta → LExpr LMonoTy IDMeta → LExpr LMonoTy IDMeta → Prop where
-| refl : ∀ σ e, StepStar σ e e
-| step : ∀ σ e e' e'', Step σ e e' → StepStar σ e' e'' → StepStar σ e e''
+inductive StepStar (F:@Factory IDMeta) (state:Scopes IDMeta)
+  : LExpr LMonoTy IDMeta → LExpr LMonoTy IDMeta → Prop where
+| refl : StepStar F state e e
+| step : ∀ e e' e'', Step F state e e' → StepStar F state e' e''
+        → StepStar F state e e''
 
 end Lambda
